L1 and L2 instances are back, and L3_L3_eta_correct too

theories/L1g/instances.v
@@ -23,58 +23,41 @@ Instance WfL1gTerm: GoodTerm (Program L1g.compile.Term) :=
 Require Import SquiggleEq.UsefulTypes.
 Require Import DecidableClass.
 
-(** deal with "spine representation" of application in L1g **)
-Fixpoint Terms_list (ts:Terms) : list Term :=
-  match ts with
-    | tnil => nil
-    | tcons u us => cons u (Terms_list us)
-  end.
-
-Inductive WFapps_list: list Term -> Prop :=
-| WFal_nil: WFapps_list nil
-| WFal_cons: forall u us,
-    WFapp u -> WFapps_list us -> WFapps_list (cons u us).
-
 Lemma nth_pres_WFapp:
   forall (us:list Term),
-    WFapps_list us -> forall n t, List.nth_error us n = Some t -> WFapp t.
+    WFapps us -> forall n t, List.nth_error us n = Some t -> WFapp t.
 Proof.
   induction 1; destruct n; intros.
   - discriminate.
   - cbn in H. discriminate.
   - cbn in H1. myInjection H1. assumption.
-  - cbn in H1. eapply IHWFapps_list. eassumption.
+  - cbn in H1. eapply IHWFapps. eassumption.
 Qed.
 
-Lemma WFapps_WFapps_list:
-  forall (ts:Terms), WFapps ts -> WFapps_list (Terms_list ts).
-Proof.
-  induction 1.
-  - constructor.
-  - constructor; assumption.
-Qed.
-    
 Function flattenApp (t:Term): (Term * (list Term)) :=
   match t with
-    | TApp fn arg args => (fn, cons arg (Terms_list args))
+    | TApp fn arg =>
+      let '(fn, args) := flattenApp fn in
+      (fn, args ++ [arg])
     | s => (s, nil)
   end.
 
 Lemma args_pres_WFapp:
   forall (t:Term), L1g.term.WFapp t ->
-       WFapp (fst (flattenApp t)) /\ WFapps_list (snd (flattenApp t)).
+       WFapp (fst (flattenApp t)) /\ WFapps (snd (flattenApp t)).
 Proof.
   induction 1; cbn; intros; repeat econstructor; try assumption.
-  - eapply WFapps_WFapps_list. assumption.
+  - destruct (flattenApp fn). intuition.
+  - destruct (flattenApp fn); simpl in *.
+    apply append_pres_WFapps; intuition.
 Qed.
-
 
 Global Instance QuestionHeadL1gTerm: QuestionHead (Program L1g.compile.Term) :=
   fun q t =>
     match q, fst (flattenApp (main t)) with
       | Cnstr ind ci, TConstruct ind2 ci2 _ _ =>
         andb (decide (ind=ind2)) (decide (ci=ci2))
-      | Abs, TLambda _ _ _ => true
+      | Abs, TLambda _ _ => true
       | _, _ => false 
     end.
 
@@ -94,28 +77,25 @@ Instance certiL1g: CerticoqLanguage (Program L1g.compile.Term):= {}.
 
 Local Generalizable Variable Lj.
 
-Definition translateTo `{CerticoqTranslation (Program L1g.compile.Term) Lj}
+Definition translateTo `{F:utils.Fuel} `{CerticoqTranslation (Program L1g.compile.Term) Lj}
   (p:Template.Ast.program): exception Lj :=
   let l1g:= L1g.compile.program_Program p in
-  match l1g with
-  | Some t => translate (Program L1g.compile.Term) Lj t
-  | None => Exc "Could not translate from Ast to L1g"
-  end.
+  translate (Program L1g.compile.Term) Lj l1g.
 
-Arguments translateTo Lj {H} p.
+Arguments translateTo {F} Lj {H} p.
 
 Require Import certiClasses.
 
-Definition ctranslateTo {Term Value BigStep WF QH ObsS } 
+Definition ctranslateTo `{F:utils.Fuel} {Term Value BigStep WF QH ObsS }
   (Lj: @CerticoqLanguage Term Value BigStep WF QH ObsS)
    `{CerticoqTranslation (Program L1g.compile.Term) (cTerm Lj)}
   : Template.Ast.program -> exception (cTerm Lj) :=
   translateTo (cTerm Lj).
 
-Arguments ctranslateTo {Term0} {Value} {BigStep} {WF} {QH} {ObsS} Lj {H} p.
+Arguments ctranslateTo {F} {Term0} {Value} {BigStep} {WF} {QH} {ObsS} Lj {H} p.
 
 
-Definition ctranslateEval {Term Value BigStep WF QH ObsS } 
+Definition ctranslateEval `{F:utils.Fuel} {Term Value BigStep WF QH ObsS }
   (Lj: @CerticoqLanguage Term Value BigStep WF QH ObsS)
    `{CerticoqTranslation (Program L1g.compile.Term) (cTerm Lj)}
    `{BigStepOpSemExec (cTerm Lj) (cValue Lj)}
@@ -125,4 +105,4 @@ Definition ctranslateEval {Term Value BigStep WF QH ObsS }
   | Exc s => Error s None 
   end.
 
-Arguments ctranslateEval {Term0} {Value} {BigStep} {WF} {QH} {ObsS} Lj {H} {H0} p n.
+Arguments ctranslateEval {F} {Term0} {Value} {BigStep} {WF} {QH} {ObsS} Lj {H} {H0} p n.
