theories/L2k_noCnstrParams/instances.v
@@ -3,7 +3,7 @@ Require Import L2k.wcbvEval.
 Require Import L2k.term.
 Require Import certiClasses.
 Require Import Common.Common.
-Require Import L2.instances.
+Require Import L1g.instances.
 Require Import certiClasses2.
 Require Import L2k.stripEvalCommute.
 
@@ -47,7 +47,7 @@ Defined.
 Global Instance certiL2k: CerticoqLanguage (Program L2k.compile.Term).
 
 Instance certiL2_to_L2k: 
-  CerticoqTotalTranslation (Program L2d.compile.Term)
+  CerticoqTotalTranslation (Program L1g.compile.Term)
                            (Program L2k.compile.Term) :=
   stripProgram.
 
