theories/L4_deBruijn/instances.v
@@ -1,7 +1,7 @@
 Require Import L4.expression.
 Require Import certiClasses.
 Require Import Common.Common.
-Require Import L3.compile.
+Require Import L2k.compile.
 Require Import L4.L3_to_L4.
 Require Import L4.L3_to_L3_eta.
 Require Import L4.L3_eta_crct.
